Semantics/KnasterTarski.lean
@@ -3,57 +3,47 @@ import Semantics.Set
 -- Concrete Semantics with Isabelle
 -- 10.4.1 The Knaster-Tarski Fixpoint Theorem on Sets
 
--- define a partial order
+/-
+## Complete lattices
+-/
+
 class PartialOrder (α: Type) extends LE α, LT α where
   le_refl: ∀a: α, a <= a
   le_trans: ∀{{a b c: α}}, a <= b -> b <= c -> a <= c
-  le_iff_le_not_le: ∀{{a b: α}}, a < b <-> a <= b ∧ ¬(b <= a)
+  lt_iff_le_not_le: ∀{{a b: α}}, a < b <-> a <= b ∧ ¬(b <= a)
   le_antisymm: ∀{{a b: α}}, a <= b -> b <= a -> a = b
 
-theorem PartialOrder.le_rfl [PartialOrder α] {a: α}:
-  a <= a :=
-  le_refl a
-
-theorem Set.le_def (a b : Set α) :
-  a <= b <-> a ⊆ b := Iff.rfl
-
-instance Set.LT (α: Type): LT (Set α) := ⟨fun a b => a ⊆ b ∧ a ≠ b⟩
-
-theorem Set.lt_def (a b : Set α):
-  a < b <-> a ⊆ b ∧ a ≠ b :=
-  Iff.rfl
-
-instance Set.partialOrder: PartialOrder (Set α) :=
-  {
-    le := fun a b => a ⊆ b,
-    lt := fun a b => a ⊆ b ∧ a ≠ b,
-    le_refl := fun _a _b => id,
-    le_antisymm := fun _a _b => Subset.antisymm,
-    le_iff_le_not_le := fun _a _b =>
-      ⟨fun ⟨hl, hr⟩ => ⟨hl, (hr $ Subset.antisymm hl .)⟩,
-        fun ⟨hl, hr⟩ => ⟨hl, (hr $ Subset.from_eq $ Eq.symm .)⟩⟩
-    le_trans := fun _a _b _c => Subset.trans
-  }
+@[refl]
+theorem PartialOrder.le_rfl [PartialOrder α] {a: α}: a <= a := le_refl a
 
 class CompleteLattice (α: Type) extends PartialOrder α where
   Inf: Set α -> α
   Inf_le: ∀{{s: Set α}}, ∀x ∈ s, Inf s <= x
   le_Inf: ∀{{s: Set α}} {{a: α}}, (∀b ∈ s, a <= b) -> a <= Inf s
 
-theorem inf_unique [CompleteLattice α]
-  (s: Set α) (a b: α)
-  (h: CompleteLattice.Inf s = a) (h': CompleteLattice.Inf s = b):
-  a = b :=
+theorem inf_unique [CompleteLattice α] (s: Set α) (a b: α)
+  (h: CompleteLattice.Inf s = a) (h': CompleteLattice.Inf s = b): a = b :=
   PartialOrder.le_antisymm
-    (h ▸ h' ▸ PartialOrder.le_refl b)
-    (h' ▸ h ▸ PartialOrder.le_refl a)
+    (h ▸ h' ▸ PartialOrder.le_rfl)
+    (h' ▸ h ▸ PartialOrder.le_rfl)
 
-instance Set.completeLattice: CompleteLattice (Set α) :=
-  {
-    Inf := fun aa => {x | ∀a ∈ aa, x ∈ a},
-    Inf_le := fun _ x hx _ ha => ha x hx,
-    le_Inf := fun _ _ h _ hb _ hd => h _ hd hb
-  }
+/-
+## Set instances
+-/
+
+instance Set.completeLattice: CompleteLattice (Set α) := {
+  le := (. ⊆ .),
+  lt := (. ⊂ .),
+  le_refl := fun _a _b => id,
+  le_antisymm := fun _a _b => Subset.antisymm,
+  lt_iff_le_not_le := fun _a _b =>
+    ⟨fun ⟨hl, hr⟩ => ⟨hl, (hr $ Subset.antisymm hl .)⟩,
+      fun ⟨hl, hr⟩ => ⟨hl, (hr $ Subset.from_eq $ Eq.symm .)⟩⟩
+  le_trans := fun _a _b _c => Subset.trans
+  Inf := fun a => {x | ∀b ∈ a, x ∈ b},
+  Inf_le := fun _ x hx _ ha => ha x hx,
+  le_Inf := fun _ _ h _ hb _ hd => h _ hd hb
+}
 
 /-
 ## Least Fixed Points
@@ -61,17 +51,18 @@ instance Set.completeLattice: CompleteLattice (Set α) :=
 
 namespace Fix
 
-def lfp [CompleteLattice α]
-  (f: α -> α): α :=
+def pre_fp [PartialOrder α] (f: α -> α) (a: α): Prop :=
+  f a <= a
+
+def lfp [CompleteLattice α] (f: α -> α): α :=
   CompleteLattice.Inf {a | f a <= a}
 
-theorem lfp_le [CompleteLattice α] {f: α -> α}
-  (h: f a <= a):
+theorem lfp_le [CompleteLattice α] {f: α -> α} (h: pre_fp f a):
   lfp f <= a :=
   CompleteLattice.Inf_le _ h
 
 theorem le_lfp [CompleteLattice α] {f: α -> α}
-  (h: ∀a', f a' <= a' -> a <= a'):
+  (h: ∀a', pre_fp f a' -> a <= a'):
   a <= lfp f :=
   CompleteLattice.le_Inf h
 
@@ -81,8 +72,7 @@ end Fix
 ## Monotonic Functions
 -/
 
-def monotone [PartialOrder α] [PartialOrder β]
-  (f: α -> β): Prop :=
+def monotone [PartialOrder α] [PartialOrder β] (f: α -> β): Prop :=
   ∀a b, a <= b -> f a <= f b
 
 theorem monotone_id [PartialOrder α]:
@@ -92,13 +82,14 @@ theorem monotone_const [PartialOrder α] [PartialOrder β]
   (b: β): monotone (fun _: α => b) :=
   fun _ _ _ => PartialOrder.le_refl b
 
-theorem monotone_union [PartialOrder α]
-  (f g: α -> Set β) (hf: monotone f) (hg: monotone g):
-  monotone (fun a => f a ∪ g a) :=
-  fun a a' ha _b hb =>
-    match hb with
-    | Or.inl h => Or.inl (hf a a' ha h)
-    | Or.inr h => Or.inr (hg a a' ha h)
+theorem Set.ite_mono (t: Set α) (hab: a ⊆ b) (hab': a' ⊆ b'):
+  ite t a a' ⊆ ite t b b' := fun _ hite =>
+  match hite with
+  | Or.inl ⟨hl, hr⟩ => Or.inl ⟨hab hl, hr⟩
+  | Or.inr ⟨hl, hr⟩ => Or.inr ⟨hab' hl, hr⟩
+
+theorem SRel.comp_mono (hfh: f ⊆ h) (hgk: g ⊆ k): f ○ g ⊆ h ○ k :=
+  fun _ ⟨z, hl, hr⟩ => ⟨z, hfh hl, hgk hr⟩
 
 /-
 ## The Knaster-Tarski Fixpoint Theorem
